First pass of entry_points. Works from Clight to x86

backend/LTL.v
@@ -18,6 +18,7 @@
 Require Import Coqlib Maps.
 Require Import AST Integers Values Events Memory Globalenvs Smallstep.
 Require Import Op Locations Conventions.
+Require Import Premain.
 
 (** * Abstract syntax *)
 
@@ -371,6 +372,7 @@ Definition pre_main (stck_sz:Z): function:=
      fn_stacksize := stck_sz;
      fn_code := pre_main_code;
      fn_entrypoint := 1%positive |}.
+
 (* loc_arguments takes a signature, 
    It generally only needs the types of arguemtns targs.
    For RISC-V, it also takes calling conventions.
@@ -380,43 +382,34 @@ Definition sig_wrapper targs:signature :=
   {| sig_args := targs;
               sig_res := None;
               sig_cc := cc_default |}.
-Definition pre_main_locset targs args: locset:=
-  build_ls_from_arguments (sig_wrapper targs) args.
 Definition arg_size (args : list typ):= Z.of_nat (Datatypes.length args).
 Definition pre_main_stack targs args: stackframe:=
   Stackframe
     (pre_main (arg_size targs))
-    Vundef                     (* no stack pointere for pre_main *)
-    (pre_main_locset targs args) (* empty environment in pre_main *)
-    nil.                       (* No continuation in pre_main *)
+    Vundef                                (* no stack pointere for pre_main *)
+    (pre_main_locset_all targs args) (* empty environment in pre_main *)
+    nil                                   (* No continuation in pre_main *).
 Definition pre_main_staklist sig args:=
   (pre_main_stack sig args)::nil.
-Definition has_pre_main (cs:list stackframe):= (0 < length cs)%nat.
-Lemma has_pre_main_cons:
-  forall hd tl, has_pre_main (hd::tl).
-Proof. intros. unfold has_pre_main. simpl; omega. Qed.
-(* Move to RTL.v*)
-Lemma nil_has_pre_main:
-      has_pre_main nil -> False.
-Proof. unfold has_pre_main; simpl; omega. Qed.
 
-        
-Search Locmap.t.
 (* build_ls_from_arguments *)
 Inductive entry_point (p: program): mem -> state -> val -> list val -> Prop :=
   | entry_point_intro: 
       let ge := Genv.globalenv p in
       forall f fb m0 m1 args targs stk l,
+      let sg:= fn_sig f in
         Genv.find_funct_ptr ge fb = Some (Internal f) ->
         (*Make sure the memory is well formed *)
         globals_not_fresh ge m0 ->
         Mem.mem_wd m0 ->
         (* Allocate a stackframe, to pass arguments in the stack*)
         Mem.alloc m0 0 0  = (m1, stk) ->
-        targs = sig_args (fn_sig f) ->
+        targs = sig_args sg ->
         Val.has_type_list args targs ->
         Mem.arg_well_formed args m0 ->
-        l = build_ls_from_arguments (fn_sig f) args ->
+        (* arguments fit in the stack *)
+        bounded_args sg ->
+        l = pre_main_locset_all targs args ->
         entry_point p m0
                     (Callstate (pre_main_staklist targs args)
                                (Internal f) l m1)
