backend/Premain.v
@@ -1,0 +1,94 @@
+
+Require Import Coqlib Locations Conventions Integers.
+Require Import AST Values.
+
+
+(* Arguemnts fit in the stack *)
+Definition bounded_args (sg: signature):=
+  4 * (size_arguments sg) < Ptrofs.max_unsigned - 30.
+
+Lemma args_bound_to_stack_bound_helper:
+  forall a b,
+    let  w := (if Archi.ptr64 then 8 else 4) in
+    4 * a < b - 30 ->
+    align (align (4*a) w + w) 8 + w < b.
+Proof.
+  intros.
+  unfold align.
+  clear - H.
+  rewrite Z.mul_comm.
+  eapply Z.le_lt_trans.
+  instantiate(1:=((4 * a + w - 1) / w * w + w + 8 - 1) + w).
+  eapply Zplus_le_compat_r.
+  apply Z.mul_div_le. xomega.
+  
+  eapply Z.le_lt_trans.
+  instantiate(1:=(4 * a + w - 1) + w + 8 - 1 + w).
+  unfold Z.sub.
+  repeat eapply Zplus_le_compat_r.
+  rewrite Z.mul_comm.
+  apply Z.mul_div_le. subst w; destruct Archi.ptr64; xomega.
+  eapply Z.le_lt_trans.
+  eapply Zplus_le_compat_l.
+  reflexivity.
+  match goal with
+    |- ?lhs < _ => replace lhs with
+      (4 * a + 3 * w + 6) by xomega
+  end.
+  assert (w <= 8).
+  { subst w. match_case; xomega. }
+  eapply (Z.le_lt_trans _ (4 * a + 30)); try xomega.
+Qed.
+
+Lemma args_bound_max:
+  forall sg, 
+    bounded_args sg ->
+    let  w := (if Archi.ptr64 then 8 else 4) in
+    align (align (4*(size_arguments sg)) w + w) 8 + w < Ptrofs.max_unsigned.
+Proof. intros. apply args_bound_to_stack_bound_helper; eauto. Qed.
+
+(* Monad for rpair *)
+Section RPairMonad.
+  Variables T K:Type.
+  Variables F: T -> val -> K -> K.
+  Definition rpair_wrap (x:rpair T)(v:val) (k1: K): K:=
+    match x with
+      | One a => F a v k1
+      | Twolong a b => F b (Val.loword v) (F a ((Val.hiword v) ) k1)
+    end.
+End RPairMonad.
+Arguments rpair_wrap {_ _}.
+
+Section ZipFold.
+  Variables T1 T2 K:Type.
+  Variables F: T1 -> T2 -> K -> K.
+  Fixpoint zip_fold (ls1: list T1)(ls2: list T2)(k:K): K:=
+    match ls1, ls2 with
+    | a::ls1',b::ls2' => F a b (zip_fold ls1' ls2' k)
+    | _, _ => k
+    end.
+End ZipFold.
+Arguments zip_fold {_ _ _}.
+
+(* Build a locset for pre_main *)
+
+Definition set_outgoing (l:loc) v ls :=
+  match l with
+  | S Outgoing _ _ => Locmap.set l v ls
+  | _ => ls
+  end.
+Definition make_locset {T K} (set_func: T -> val -> K -> K) :=
+  zip_fold (rpair_wrap set_func).
+
+Definition make_locset_all:= make_locset Locmap.set.
+Definition make_locset_outgoing:= make_locset set_outgoing.
+
+Notation locset := Locmap.t.
+Definition sig_wrapper targs:signature :=
+  {| sig_args := targs; sig_res := None; sig_cc := cc_default |}.
+Definition pre_main_locset_outgoing targs args: locset:=
+  let sg:= sig_wrapper targs in
+  make_locset_outgoing (loc_arguments sg) args (Locmap.init Vundef).
+Definition pre_main_locset_all targs args: locset:=
+  let sg:= sig_wrapper targs in
+  make_locset_all (loc_arguments sg) args (Locmap.init Vundef).
