cfrontend/Clight.v
@@ -30,6 +30,7 @@ Require Import Globalenvs.
 Require Import Smallstep.
 Require Import Ctypes.
 Require Import Cop.
+Require Import Premain.
 
 (** * Abstract syntax *)
 
@@ -749,65 +750,11 @@ Inductive val_casted_list: list val -> typelist -> Prop :=
       val_casted v1 ty1 -> val_casted_list vl tyl ->
       val_casted_list (v1 :: vl) (Tcons  ty1 tyl).
 
-(* Require Import Conventions.
-
-Definition loc_arguments' l := if Archi.ptr64 then loc_arguments_64 l 0 0 0 else loc_arguments_32 l 0. *)
-
-(*NOTE: DOUBLE CHECK TARGS (it's not used right now)*)
-(*
-Old entry_point
-Inductive entry_point (ge:genv): mem -> state -> val -> list val -> Prop :=
-| initi_core:
-    forall f fb b0 f0 m0 m1 stk args targs tres,
-      Genv.find_funct_ptr ge fb = Some f ->
-      type_of_fundef f = Tfunction targs tres cc_default ->
-      globals_not_fresh ge m0 ->
-      Mem.mem_wd m0 ->
-      Mem.arg_well_formed args m0 ->
-      val_casted_list args targs ->
-      Val.has_type_list args (typlist_of_typelist targs) ->
-      (*val_casted_list_func args targs 
-                           && tys_nonvoid targs 
-                           && vals_defined args
-                           && zlt (4*(2*(Zlength args))) Int.max_unsigned = true ->*)
-      Genv.find_funct_ptr ge b0 = Some (Internal f0) ->
-      Mem.alloc m0 0 0 = (m1, stk) ->
-      entry_point ge m0 (Callstate f args
-                                   (Kcall None f0 empty_env
-                                                 (temp_bindings
-                                                    1%positive (Vptr fb Ptrofs.zero::args)) Kstop) m1) (Vptr fb Ptrofs.zero) args.*)
-
-
-(*Explain the new entry_points:
-  1. Starts one step before calling main or the spawned function,
-     this way it can create a stack to put arguments if any.
-  2. Assumes no return. Might be easy to check.
-  3.       
-
- *)
-(*
-Inductive function_entry2 ge f vargs m e le m'
-          (ge: genv)  (f: function) (vargs: list val) (m: mem) (e: env) (le: temp_env) (m': mem)
-  | function_entry2_intro:
-      list_norepet (var_names f.(fn_vars)) ->
-      list_norepet (var_names f.(fn_params)) ->
-      list_disjoint (var_names f.(fn_params)) (var_names f.(fn_temps)) ->
-      
-      alloc_variables ge empty_env m f.(fn_vars) e m' ->
-
-      bind_parameter_temps f.(fn_params) vargs (create_undef_temps f.(fn_temps)) = Some le ->
-      function_entry2 ge f vargs m e le m'.
- *)
-
-(*TODO: fill in:
- - targs tres AT
-*)
 Inductive entry_point (ge:genv): mem -> state -> val -> list val -> Prop :=
 | initi_core:
     forall f fb m0 args targs AT,
+      let sg:= signature_of_type targs type_int32s cc_default in
       Genv.find_funct_ptr ge fb = Some (Internal f) ->
-      (* Assume there are no local variables, this could change*)
-      f.(fn_vars) = nil ->
       (* The only argument is a pointer*)
       f.(fn_params) = (xH, Tpointer (Tfunction targs type_int32s  cc_default)  AT)::nil ->
       (*Make sure the memory is well formed *)
@@ -816,16 +763,10 @@ Inductive entry_point (ge:genv): mem -> state -> val -> list val -> Prop :=
       typlist_of_typelist targs =
       (map (fun x => typ_of_type (snd x)) (fn_vars f)) ->
       (* Allocate a stackframe, to pass arguments in the stack*)
-      (*Mem.alloc m0 0 0 = (m1, stk) -> *)
       Val.has_type_list args (typlist_of_typelist targs) ->
       Mem.arg_well_formed args m0 ->
       type_of_fundef (Internal f) = Tfunction targs type_int32s cc_default ->
-      (*Mem.arg_well_formed args m0 ->
-      val_casted_list args targs ->
-      val_casted_list_func args targs 
-                           && tys_nonvoid targs 
-                           && vals_defined args
-                           && zlt (4*(2*(Zlength args))) Int.max_unsigned = true ->*)
+      bounded_args sg ->
       entry_point ge m0
                   (Callstate (Internal f) args (Kstop targs) m0) (Vptr fb Ptrofs.zero) args.
 
